fixed some bugs in the paper proofs in Appendix A (Section 2.2). Proved some of them in Coq.
git-svn-id: https://webdav.seas.upenn.edu/svn/sol/vol@4262 eef5ea85-cc2e-0410-bd84-0fae1f012da8

src3.0/Transforms/vmem2reg_opt_compose_props.v
@@ -1742,18 +1742,24 @@ Section ActionGraph.
 
 Variable actions: AssocList action.
 
-Definition avertexes : V_set :=
+Definition avertexes : @V_set value :=
 fun (v:Vertex) => 
-  let '(index n) := v in 
-  n `in` dom actions \/ exists id0, In (id0, AC_vsubst (value_id n)) actions.
+let '(index val) := v in 
+match val with
+| value_id n => 
+  n `in` dom actions 
+| _ => False 
+end \/ exists id0, In (id0, AC_vsubst val) actions.
 
-Definition aarcs : A_set :=
+Definition aarcs : @A_set value :=
 fun (arc:Arc) =>
-  let '(A_ends (index n2) (index n1)) := arc in
-  In (n2, AC_vsubst (value_id n1)) actions. 
+match arc with
+| (A_ends (index (value_id id2)) (index v1)) => In (id2, AC_vsubst v1) actions
+| _ => False
+end.
 
 Definition acyclic_actions : Prop :=
-  forall (x:Vertex) (vl:V_list) (al:A_list) (Hcyc: D_path avertexes aarcs x x vl al), 
+  forall (x:Vertex) (vl:V_list) (al:A_list) (Hcyc: D_walk avertexes aarcs x x vl al), 
     vl = V_nil.
 
 End ActionGraph.
@@ -1763,7 +1769,7 @@ Lemma find_stld_pairs_block__isReachableFromEntry: forall s m fh bs
   (HuniqF: uniqFdef (fdef_intro fh bs)) pid rd actions
   (Hreach: ret rd = reachablity_analysis (fdef_intro fh bs))
   (Hfind: actions = flat_map (find_stld_pairs_block pid rd) bs),
-  forall id0 (a:avertexes actions (index id0)) (b : block),
+  forall id0 (a:avertexes actions (index (value_id id0))) (b : block),
   lookupBlockViaIDFromFdef (fdef_intro fh bs) id0 = ret b ->
   isReachableFromEntry (fdef_intro fh bs) b.
 Proof.
@@ -1883,40 +1889,129 @@ Proof.
       subst c1. simpl. auto.
 Qed.
 
-Lemma find_stld_pairs_blocks__walk_idDominates: forall s m fh bs 
+Lemma find_stld_pairs_blocks__valueDominates: forall s m fh bs 
+  (HwfF:wf_fdef s m (fdef_intro fh bs))
+  (HuniqF: uniqFdef (fdef_intro fh bs)) actions rd pid
+  (Hreach: ret rd = reachablity_analysis (fdef_intro fh bs))
+  (Hfind: actions = flat_map (find_stld_pairs_block pid rd) bs) id1 v2
+  (Hin: In (id1, AC_vsubst v2) actions),
+  valueDominates (fdef_intro fh bs) v2 (value_id id1).
+Proof.
+  intros.
+  destruct v2 as [id2|]; simpl; auto.
+  intros.
+  eapply find_stld_pairs_blocks__idDominates; eauto.
+Qed.
+
+(* go to typing_props.v *)
+Lemma idDominates_id_in_reachable_block: forall (s : system) (m : module)
+  (f : fdef) (HwfF : wf_fdef s m f) (HuniqF : uniqFdef f) (id2 : id) (id3 : id)
+  (Hreach : id_in_reachable_block f id3) (Hdom : idDominates f id2 id3),
+  id_in_reachable_block f id2.
+Proof.
+  intros.
+  unfold id_in_reachable_block in *.
+  intros.
+  unfold idDominates in *.
+  inv_mbind.
+  
+  unfold inscope_of_id in HeqR0.
+  destruct b as [l1 [ps1 cs1 tmn1]].
+  symmetry in HeqR0.
+  apply fold_left__spec in HeqR0.
+  destruct HeqR0 as [J1 [J2 J3]].
+  apply_clear J3 in Hdom.
+  assert (blockInFdefB (l1, stmts_intro ps1 cs1 tmn1) f = true) as HBinF1.
+    symmetry in HeqR. solve_blockInFdefB. 
+  assert (blockInFdefB b2 f = true) as HBinF2 by solve_blockInFdefB.
+  assert (In id2 (getStmtsLocs (snd b2))) as Hin by solve_in_list.
+  destruct Hdom as [Hdom | [sts2 [l2 [J4 [J5 J3]]]]].
+    assert (~ In id2 (getArgsIDsOfFdef f)) as Hnotin2.
+      solve_notin_getArgsIDs.
+    unfold init_scope in Hdom.
+    destruct_if; try tauto.
+    apply Hreach.
+      f_equal.
+      apply block_eq2 with (id1:=id2)(f:=f); auto.
+        simpl. xsolve_in_list.
+        apply cmds_dominates_cmd_spec in Hdom; auto.
+        xsolve_in_list.
+  
+    assert (b2 = (l2, sts2)) as EQ.
+      apply block_eq2 with (id1:=id2)(f:=f); auto.
+        solve_blockInFdefB.
+        simpl. xsolve_in_list.
+    subst.
+    assert (Some (l1, stmts_intro ps1 cs1 tmn1) = 
+            Some (l1, stmts_intro ps1 cs1 tmn1)) as EQ by auto.
+    apply Hreach in EQ.
+    assert (strict_domination f l2 l1) as J.
+      eapply sdom_is_sound with (s3:=stmts_intro ps1 cs1 tmn1); eauto 1.
+        apply set_diff_elim1 in J4; auto.
+    apply DecDom.sdom_reachable in J; auto.
+Qed.
+
+(* go to typing_props.v *)
+Lemma valueDominates_trans: forall s m f (HwfF:wf_fdef s m f)
+  (HuniqF: uniqFdef f) v1 v2 v3
+  (Hdom1: valueDominates f v1 v2) (Hdom2: valueDominates f v2 v3),
+  valueDominates f v1 v3.
+Proof.
+  intros.
+  destruct v1 as [id1|]; auto.
+  destruct v2 as [id2|]; tinv Hdom1.
+  destruct v3 as [id3|]; tinv Hdom2.
+  simpl in *.
+  intro Hreach.
+  eapply idDominates_trans; eauto.
+    apply Hdom1.
+    assert (Hdom:=Hreach). apply Hdom2 in Hdom. 
+    eapply idDominates_id_in_reachable_block; eauto.
+Qed.
+
+Lemma D_walk_head_inv : forall acs v1 v2 vl al
+  (Hw: D_walk (avertexes acs) (aarcs acs) v1 v2 vl al),
+  (v1 = v2 /\ vl = V_nil /\ al = A_nil) \/ exists id1, v1 = index (value_id id1).
+Proof.
+  intros.
+  inv Hw; auto.
+  destruct v1 as [[]]; tinv H1; eauto.
+Qed.
+
+Lemma find_stld_pairs_blocks__walk_valueDominates: forall s m fh bs 
   (HwfF:wf_fdef s m (fdef_intro fh bs))
   (HuniqF: uniqFdef (fdef_intro fh bs)) actions rd pid
   (Hreach: ret rd = reachablity_analysis (fdef_intro fh bs))
   (Hfind: actions = flat_map (find_stld_pairs_block pid rd) bs)
-  id1 id2 vl al (Hnnil: vl <> V_nil)
-  (Hw: D_walk (avertexes actions) (aarcs actions) (index id1) (index id2) vl al),
-  idDominates (fdef_intro fh bs) id2 id1.
+  id1 v2 vl al (Hnnil: vl <> V_nil)
+  (Hw: D_walk (avertexes actions) (aarcs actions) 
+         (index (value_id id1)) (index v2) vl al),
+  valueDominates (fdef_intro fh bs) v2 (value_id id1).
 Proof.
   intros.
   remember (avertexes actions) as V.
   remember (aarcs actions) as A.
-  remember (index id1) as x.
-  remember (index id2) as y.
+  remember (index (value_id id1)) as x.
+  remember (index v2) as y.
   generalize dependent id1.
-  generalize dependent id2.
+  generalize dependent v2.
   induction Hw; intros; subst.
   Case "1".
     congruence.
   Case "2".
-    destruct y as [id3].
-    eapply find_stld_pairs_blocks__idDominates in H0; eauto.
-    destruct vl as [|v' vl].
-    SCase "2.1".
-      inv Hw; auto.
-    SCase "2.2".
-      eapply idDominates_trans; eauto 1.
-      SSCase "A".
-        apply IHHw; auto. 
-          intro J. inv J.
-      SSCase "B".
-        eapply find_stld_pairs_block__isReachableFromEntry with (pid:=pid); 
-          eauto.
-          simpl_env. auto.
+    destruct y as [v3].
+    match goal with
+    | H0: aarcs _ _ |- _ =>
+      eapply find_stld_pairs_blocks__valueDominates in H0; eauto 1
+    end.
+    destruct vl as [|v' vl]; inv Hw; auto.
+    match goal with
+    | H8 : aarcs _ (A_ends (index ?v3) _) |- _ =>
+      destruct v3 as [id3|]; tinv H8
+    end.
+    eapply valueDominates_trans; eauto 1.
+      apply IHHw; auto. 
+        intro J. inv J.
 Qed.
 
 Lemma find_stld_pairs_blocks_acyclic: forall s m fh bs 
@@ -1934,14 +2029,21 @@ Proof.
     with (pid:=pid)(rd:=rd)(actions:=flat_map (find_stld_pairs_block pid rd) bs)
     in Hwfa; auto.
   destruct vl as [|v vl]; auto.
-  assert (Hin:=Hcyc). apply DP_endx_inv in Hin.
-  apply D_path_isa_walk in Hcyc. 
-  destruct x as [id0].
-  eapply find_stld_pairs_blocks__walk_idDominates in Hcyc; eauto.
+  assert (Hin:=Hcyc). apply DW_endx_inv in Hin.
+  assert (J:=Hcyc).
+  apply D_walk_head_inv in J.
+  destruct J as [[EQ1 [EQ2 EQ3]]|[id0 EQ]]; subst; try congruence.
+  eapply find_stld_pairs_blocks__walk_valueDominates in Hcyc; eauto.
   Case "1".
-    eapply idDominates_acyclic in Hcyc; eauto.
+    simpl in Hcyc.
+    assert (id_in_reachable_block (fdef_intro fh bs) id0) as Hreach'.
+      unfold id_in_reachable_block.
+      intros.
+      eapply find_stld_pairs_block__isReachableFromEntry in Hin; eauto.     
+    apply Hcyc in Hreach'.
+    eapply idDominates_acyclic in Hreach'; eauto.
     SCase "1.1".
-      inv Hcyc.
+      inv Hreach'.
     SCase "1.2".
       intros.
       eapply find_stld_pairs_block__isReachableFromEntry in Hin; eauto.     
@@ -1981,7 +2083,7 @@ Proof.
 Qed.
 
 Definition nonused_in_Vertex (id0:id) (v:Vertex) : Prop :=
-  let 'index id' := v in id0 <> id'.
+  let 'index v' := v in used_in_value id0 v' = false.
 
 Definition nonused_in_V_list (id0:id) (vl:V_list) : Prop :=
   Forall (nonused_in_Vertex id0) vl.
@@ -1992,16 +2094,17 @@ Lemma nonused__subst_avertexex: forall id0 ac0 (acs:AssocList action) v
   avertexes acs' v.
 Proof.
   unfold avertexes. 
-  intros. subst. destruct v as [id1].
+  intros. subst. 
+  destruct v as [v].
   destruct Ha as [Ha | [id2 Ha]].
-    left.   
-    assert (J:=list_subst_actions__dom id0 ac0 acs).
-    fsetdec.
+    destruct v as [id1|cst1]; auto.
+      left.   
+      assert (J:=list_subst_actions__dom id0 ac0 acs).
+      fsetdec.
 
     right. 
     exists id2.
     apply nonused__in_subst_actions; auto.
-    simpl in *. destruct_dec.
 Qed.
 
 Lemma Forall_inv' : forall A P (a:A) l, Forall P (a :: l) -> Forall P l.
@@ -2015,15 +2118,18 @@ Lemma nonused__subst_aarcs: forall id0 ac0 (acs:AssocList action) x y
   (Heq: acs' = (ListComposedPass.subst_actions id0 ac0 acs)),
   aarcs acs' (A_ends x y).
 Proof.
-  intros. destruct x as [x1]. destruct y as [y1]. simpl in *.
+  intros. 
+  destruct x as [[id1|cst1]]; tinv Ha.
+  destruct y as [y1]. simpl in *.
   subst.
   apply nonused__in_subst_actions; auto.
-    simpl. destruct_dec.
 Qed.
 
 Definition Vertex_in_action_dom (v:Vertex) (acs:AssocList action) : Prop :=
-let 'index id0 := v in
-id0 `in` dom acs.
+match v with
+| index (value_id id0) => id0 `in` dom acs
+| _ => False
+end.
 
 Lemma dom__subst_avertexex: forall id0 ac0 (acs:AssocList action) v
   (Hdom: Vertex_in_action_dom v acs) acs' 
@@ -2031,7 +2137,7 @@ Lemma dom__subst_avertexex: forall id0 ac0 (acs:AssocList action) v
   avertexes acs' v.
 Proof.
   unfold avertexes. 
-  intros. subst. destruct v as [id1].
+  intros. subst. destruct v as [[id1|cst1]]; tinv Hdom.
   left.  simpl in *.
   assert (J:=list_subst_actions__dom id0 ac0 acs).
   fsetdec.
@@ -2098,75 +2204,538 @@ Proof.
     ].
 Qed.
 
-Definition V_list__in__actions (al:E_list) (acs:AssocList action) : Prop :=
-forall x y (Hin: In (E_ends (index x) (index y)) al),
-  In (x, AC_vsubst (value_id y)) acs.
-
-Definition actions_incl (acs1 acs2:AssocList action) : Set :=
-forall vl1 al1 v1 v2
-  (Hw: D_walk (avertexes acs1) (aarcs acs1) v1 v2 vl1 al1),
-  exists vl2, exists al2, D_walk (avertexes acs2) (aarcs acs2) v1 v2 vl2 al2.
-
-Fixpoint can_only_be_at_the_end (v:@Vertex atom) (vs:V_list) : Prop :=
-match vs with
-| nil => True
-| _::nil => True
-| v'::vs' => v' <> v /\ can_only_be_at_the_end v vs'
+Definition end_of_actions (v:@Vertex value) (acs:AssocList action) : Prop :=
+let '(index v0) := v in
+match v0 with
+| value_id id0 => lookupAL _ acs id0 = None
+| _ => True
 end.
 
-Definition wf_D_walk v a x0 y0 vl al z0 :=
-  D_walk v a x0 y0 vl al /\
-  can_only_be_at_the_end z0 vl.
+Definition actions_end_imply (acs1 acs2:AssocList action) : Prop :=
+forall vl1 al1 v1 v2
+  (Hw: D_walk (avertexes acs1) (aarcs acs1) v1 v2 vl1 al1)
+  (Hend: end_of_actions v2 acs1),
+  exists vl2, exists al2, 
+    D_walk (avertexes acs2) (aarcs acs2) v1 v2 vl2 al2 /\
+    end_of_actions v2 acs2.
 
-Inductive connected_dwalks_tail (v:V_set) (a:A_set) (z0 y0:@Vertex atom):
-  list ((@V_list atom)*(@A_list atom)) -> Prop :=
-| CDT_nil : z0 = y0 -> connected_dwalks_tail v a z0 y0 nil
-| CDT_single : forall vl al,
-               wf_D_walk v a z0 y0 vl al z0 ->
-               connected_dwalks_tail v a z0 y0 ((vl, al)::nil)
-| CDT_cons : forall vl al wks,
-    wf_D_walk v a z0 z0 vl al z0 ->
-    connected_dwalks_tail v a z0 y0 wks ->
-    connected_dwalks_tail v a z0 y0 ((vl, al)::wks)
+Inductive dwalks : Set :=
+| DW_nil : dwalks
+| DW_single : @V_list value -> @A_list value -> dwalks
+| DW_more : 
+    @V_list value -> @Vertex value -> @A_list value ->
+    list (@V_list value * @Vertex value  * @A_list value) ->
+    @V_list value ->  @A_list value ->
+    dwalks.
+
+Definition V_list_doesnt_contain (v:@Vertex value) (vl:V_list) : Prop :=
+Forall (fun v' => v' <> v) vl.
+
+(*
+   There is a path from x0 to y0. We want to substitute z0 by v0.
+   We partition the path in the following.
+   o fine if the path is empty
+   o the path (except the end) does not contain z0
+   o otherwise
+      x0 .. v1 z0 v0 .. v1 z0 v0 ... ... ... z0 v0 ... y0
+*)
+Inductive wf_dwalks (v:V_set) (a:A_set) (vl: @V_list value) (al: @A_list value) 
+  (x0 y0 z0 v0:@Vertex value) : dwalks -> Prop :=
+| WDW_nil : 
+    x0 = y0 -> vl = V_nil -> al = A_nil ->
+    wf_dwalks v a vl al x0 y0 z0 v0 DW_nil
+| WDW_single :
+    D_walk v a x0 y0 vl al ->
+    vl <> V_nil ->
+    V_list_doesnt_contain z0 (removelast vl) ->
+    wf_dwalks v a vl al x0 y0 z0 v0 (DW_single vl al)
+| WDW_more : forall vl1 v1 al1 vals2 vl3 al3,
+    (* head *)
+    D_walk v a x0 v1 vl1 al1 ->
+    D_walk v a v1 z0 [z0] [A_ends v1 z0] ->
+    V_list_doesnt_contain z0 vl1 ->
+    (* middles *)
+    Forall (fun val2 => 
+            let '(vl2, v2, al2) := val2 in 
+            D_walk v a z0 v0 [v0] [A_ends z0 v0] /\
+            D_walk v a v0 v2 vl2 al2 /\
+            D_walk v a v2 z0 [z0] [A_ends v2 z0] /\
+            V_list_doesnt_contain z0 vl2) vals2 ->
+    (* end *)
+    D_walk v a z0 v0 [v0] [A_ends z0 v0] ->
+    D_walk v a v0 y0 vl3 al3 ->    
+    V_list_doesnt_contain z0 (removelast vl1) ->
+    (* sum *)
+    fold_left (fun acc val2 => 
+               let '(vl2, _, al2) := val2 in 
+               acc ++ v0 :: vl2 ++ [z0]) vals2 (vl1 ++ [z0]) ++ (v0::vl3) = vl ->
+    fold_left (fun acc val2 => 
+               let '(vl2, v2, al2) := val2 in 
+               acc ++ A_ends z0 v0 :: al2 ++ [A_ends v2 z0]) 
+      vals2 (al1 ++ [A_ends v1 z0]) ++ (A_ends z0 v0 ::al3) = al ->
+    wf_dwalks v a vl al x0 y0 z0 v0 (DW_more vl1 v1 al1 vals2 vl3 al3)
 .
 
-Definition connected_dwalks (v:V_set) (a:A_set) (x0 z0 y0:Vertex) 
-  (wks: list ((@V_list atom)*A_list)) : Prop :=
-match wks with
-| nil => True
-| (vl, al)::nil => wf_D_walk v a x0 y0 vl al z0
-| (vl, al)::wks' => 
-    wf_D_walk v a x0 z0 vl al z0 /\ connected_dwalks_tail v a z0 y0 wks'
+Lemma generate_connected_dwalks: forall acs x0 y0 vl al z0 v0,
+  uniq acs ->
+  D_walk (avertexes acs) (aarcs acs) x0 y0 vl al ->
+  exists wks, 
+    wf_dwalks (avertexes acs) (aarcs acs) vl al x0 y0 z0 v0 wks.
+Admitted.
+
+(*
+  Given a path
+      x0 .. v1 z0 v0 .. v1 z0 v0 ... ... ... z0 v0 ... y0
+  the new path after substitution is
+      x0 .. v1    v0 .. v1    v0 ... ... ...    v0 ... y0
+*)
+Definition dwalks_to_walk v0 (dw:dwalks): @V_list value * @A_list value :=
+match dw with
+| DW_nil => (V_nil, A_nil)
+| DW_single vl al => (vl, al)
+| DW_more vl1 v1 al1 vals2 vl3 al3 =>
+    (fold_left (fun acc val2 => 
+                let '(vl2, _, al2) := val2 in 
+                acc ++ v0 :: vl2) vals2 vl1 ++ (v0::vl3),
+     fold_left (fun acc val2 => 
+                let '(vl2, v2, al2) := val2 in 
+                acc ++ al2 ++ [A_ends v2 v0]) 
+       vals2 (al1 ++ [A_ends v1 v0]) ++ al3)
 end.
 
-Definition dwalk_eq_dwalks vl al 
-  (wks: list ((@V_list atom)*(@A_list atom))) : Prop :=
-let '(vls, als) := List.split wks in
-fold_left (@app Vertex) vls nil = vl /\
-fold_left (@app Arc) als nil = al.
-
-Definition partitioned_dwalks (v:V_set) (a:A_set) (x0 z0 y0:Vertex) 
-  vl al (wks: list ((@V_list atom)*A_list)) : Prop :=
-connected_dwalks v a x0 z0 y0 wks /\
-dwalk_eq_dwalks vl al wks.
-
-Lemma generate_connected_dwalks: forall v a x0 y0 vl al z0,
-  D_walk v a x0 y0 vl al ->
-  exists wks, partitioned_dwalks v a x0 z0 y0 vl al wks.
-Admitted.
-
-Lemma subst_actions_incl: forall acs id0 ac0 (Huniq: uniq acs)
+Lemma subst_actions_end_imply: forall acs id0 ac0 (Huniq: uniq acs)
   (Hin: In (id0, ac0) acs),
-  actions_incl acs (ListComposedPass.subst_actions id0 ac0 acs).
+  actions_end_imply acs (ListComposedPass.subst_actions id0 ac0 acs).
 Proof.
-  unfold actions_incl.
+  unfold actions_end_imply.
   intros.
-  apply generate_connected_dwalks with (z0:=index id0) in Hw.
-  destruct Hw as [wks [J1 J2]].
-
-
-Admitted.
+  remember (action2value ac0) as ov.
+  destruct ov as [v|].
+  Case "ov=Some v".
+    apply generate_connected_dwalks 
+      with (z0:=index (value_id id0))(v0:=index v) in Hw; auto.
+    destruct Hw as [wks J].
+    destruct (dwalks_to_walk (index v) wks) as [vl' al'].
+    exists vl'. exists al'.
+    admit. (* by nonused__subst_actions_dwalk' *)
+  Case "ov=None".
+    unfold ListComposedPass.subst_actions.
+    rewrite <- Heqov. eauto.
+Qed.
   
+Definition A_list__in__actions (al:A_list) (acs:AssocList action) : Prop :=
+forall id0 v (Hin: In (A_ends (index (value_id id0)) (index v)) al),
+  In (id0, AC_vsubst v) acs.
+
+(*
+   There is a path from x0 to y0, in which z0 was substituted by v0.
+   We partition the path in the following.
+   o fine if the path is empty
+   o the path (except the end) does not contain fresh (z0',v0).
+   o otherwise
+      x0 .. z0' v0 .. z1' v0 ... ... ... zn' v0 ... y0
+      where (z0', v0) is not in the original graph.
+*)
+Inductive wf_inv_dwalks (v:V_set) (a:A_set) (acs:AssocList action)
+  (vl: @V_list value) (al: @A_list value) 
+  (x0 y0 v0:@Vertex value) : dwalks -> Prop :=
+| WIDW_nil : 
+    x0 = y0 -> vl = V_nil -> al = A_nil ->
+    wf_inv_dwalks v a acs vl al x0 y0 v0 DW_nil
+| WIDW_single :
+    D_walk v a x0 y0 vl al ->
+    vl <> V_nil ->
+    A_list__in__actions al acs ->
+    wf_inv_dwalks v a acs vl al x0 y0 v0 (DW_single vl al)
+| WIDW_more : forall vl1 v1 al1 vals2 vl3 al3,
+    (* head *)
+    D_walk v a x0 v1 vl1 al1 ->
+    D_walk v a v1 v0 [v0] [A_ends v1 v0] ->
+    A_list__in__actions al1 acs ->
+    (* middles *)
+    Forall (fun val2 => 
+            let '(vl2, v2, al2) := val2 in 
+            D_walk v a v0 v2 vl2 al2 /\
+            D_walk v a v2 v0 [v0] [A_ends v2 v0] /\
+            A_list__in__actions al2 acs) vals2 ->
+    (* end *)
+    D_walk v a v0 y0 vl3 al3 ->    
+    A_list__in__actions al3 acs ->
+    (* sum *)
+    fold_left (fun acc val2 => 
+               let '(vl2, _, al2) := val2 in 
+               acc ++ vl2 ++ [v0]) vals2 (vl1 ++ [v0]) ++ vl3 = vl ->
+    fold_left (fun acc val2 => 
+               let '(vl2, v2, al2) := val2 in 
+               acc ++ al2 ++ [A_ends v2 v0]) 
+      vals2 (al1 ++ [A_ends v1 v0]) ++ al3 = al ->
+    wf_inv_dwalks v a acs vl al x0 y0 v0 (DW_more vl1 v1 al1 vals2 vl3 al3)
+.
+
+Lemma generate_connected_inv_dwalks: forall acs x0 y0 vl al id0 ac0 v0 acs'
+  (Hsome: Some v0 = action2value ac0)
+  (Heq: acs' = (ListComposedPass.subst_actions id0 ac0 acs)),
+  uniq acs ->
+  D_walk (avertexes acs') (aarcs acs') x0 y0 vl al ->
+  exists wks, 
+    wf_inv_dwalks (avertexes acs) (aarcs acs) acs vl al x0 y0 (index v0) wks.
+Admitted.
+
+(*
+  Given a path
+      x0 .. v1    v0 .. v1    v0 ... ... ...    v0 ... y0
+  the new path before substitution is
+      x0 .. v1 z0 v0 .. v1 z0 v0 ... ... ... z0 v0 ... y0
+*)
+Definition inv_dwalks_to_walk z0 v0 (dw:dwalks): @V_list value * @A_list value :=
+match dw with
+| DW_nil => (V_nil, A_nil)
+| DW_single vl al => (vl, al)
+| DW_more vl1 v1 al1 vals2 vl3 al3 =>
+    (fold_left (fun acc val2 => 
+                let '(vl2, _, al2) := val2 in 
+                acc ++ z0 :: v0 :: vl2) vals2 vl1 ++ (z0 :: v0::vl3),
+     fold_left (fun acc val2 => 
+                let '(vl2, v2, al2) := val2 in 
+                acc ++ al2 ++ A_ends v2 z0 :: [A_ends z0 v0]) 
+       vals2 (al1 ++ A_ends v1 z0 :: [A_ends z0 v0]) ++ al3)
+end.
+
+Definition actions_len_imply (acs1 acs2:AssocList action) : Prop :=
+forall vl1 al1 v1 v2
+  (Hw: D_walk (avertexes acs1) (aarcs acs1) v1 v2 vl1 al1),
+  exists vl2, exists al2, 
+    D_walk (avertexes acs2) (aarcs acs2) v1 v2 vl2 al2 /\
+    (length vl2 >= length vl1)%nat.
+
+Lemma subst_actions_len_imply_inv: forall acs id0 ac0 (Huniq: uniq acs)
+  (Hin: In (id0, ac0) acs),
+  actions_len_imply (ListComposedPass.subst_actions id0 ac0 acs) acs.
+Proof.
+  unfold actions_len_imply.
+  intros.
+  remember (action2value ac0) as ov.
+  destruct ov as [v0|].
+  Case "ov=Some v".
+    apply generate_connected_inv_dwalks
+      with (id0:=id0)(v0:=v0)(ac0:=ac0)(acs:=acs) in Hw; auto.
+    destruct Hw as [wks J].
+    destruct (inv_dwalks_to_walk (index (value_id id0)) (index v0) wks) 
+      as [vl' al'].
+    exists vl'. exists al'.
+    admit. (* subst_actions_inv *)
+  Case "ov=None".
+    unfold ListComposedPass.subst_actions in *.
+    rewrite <- Heqov in *. eauto.
+Qed.
+
+Lemma subst_actions_end_of_actions_inv: forall v2 id0 ac0 acs
+  (Hend: end_of_actions v2 (ListComposedPass.subst_actions id0 ac0 acs)),
+  end_of_actions v2 acs.
+Proof.
+  intros.
+  assert (J:=list_subst_actions__dom id0 ac0 acs).
+  unfold ListComposedPass.subst_actions in *.
+  intros.
+  remember (action2value ac0) as ov0.
+  destruct ov0 as [v0|]; auto.
+  unfold end_of_actions in *.
+  destruct v2 as [[vid|]]; auto.
+  apply lookupAL_None_notindom in Hend.
+  apply notin_lookupAL_None. fsetdec.
+Qed.
+
+Lemma subst_actions_inv_end_incl: forall acs id0 ac0 (Huniq: uniq acs)
+  (Hin: In (id0, ac0) acs),
+  actions_end_imply (ListComposedPass.subst_actions id0 ac0 acs) acs.
+Proof.
+  intros.
+  apply subst_actions_len_imply_inv in Hin; auto.
+  unfold actions_end_imply. unfold actions_len_imply in *.
+  intros.
+  apply Hin in Hw.
+  destruct Hw as [vl2 [al2 [Hw Hlen]]].
+  exists vl2. exists al2.
+  split; eauto using subst_actions_end_of_actions_inv.
+Qed.
+
+Definition actions_eq (acs1 acs2:AssocList action) : Prop :=
+actions_end_imply acs1 acs2 /\ actions_end_imply acs2 acs1.
+
+Lemma subst_actions_eq: forall acs id0 ac0 (Huniq: uniq acs)
+  (Hin: In (id0, ac0) acs),
+  actions_eq acs (ListComposedPass.subst_actions id0 ac0 acs).
+Proof.
+  intros.
+  split.
+    apply subst_actions_end_imply; auto.
+    apply subst_actions_inv_end_incl; auto.
+Qed.
+
+Lemma len_le_zero__nil: forall A (vl:@list A) (Hlen: (0 >= length vl)%nat),
+  vl = nil.
+Proof.
+  intros.
+  destruct vl; auto.
+    simpl in *. contradict Hlen. omega.
+Qed.
+
+Lemma subst_actions_acyclic: forall acs id0 ac0 (Huniq: uniq acs)
+  (Hin: In (id0, ac0) acs) (Hacyc: acyclic_actions acs),
+  acyclic_actions (ListComposedPass.subst_actions id0 ac0 acs).
+Proof.
+  unfold acyclic_actions.
+  intros. 
+  apply subst_actions_len_imply_inv in Hcyc; auto.
+  destruct Hcyc as [vl2 [al2 [Hw Hlen]]].
+  apply Hacyc in Hw. subst. 
+  eapply len_le_zero__nil; eauto.
+Qed.
+
+Definition in_codom_of_actions (id0:id) (acs:AssocList action) : Prop :=
+Exists (fun elt =>
+        let '(_, ac) := elt in
+        match action2value ac with
+        | Some v => used_in_value id0 v
+        | _ => False
+        end) acs.
+
+Definition notin_codom_of_actions (id0:id) (acs:AssocList action) : Prop :=
+Forall (fun elt =>
+        let '(_, ac) := elt in
+        match action2value ac with
+        | Some v => used_in_value id0 v = false
+        | _ => True
+        end) acs.
+
+Lemma nonused_in_action__notin_codom_of_actions: forall id0 ac0 acs v0
+  (Hnuse: used_in_action id0 ac0 = false) (Hsome: Some v0 = action2value ac0),
+  notin_codom_of_actions id0 (ListComposedPass.subst_actions id0 ac0 acs).
+Proof.
+  unfold ListComposedPass.subst_actions.
+  intros. rewrite <- Hsome.
+  unfold notin_codom_of_actions.
+  induction acs as [|[id1 ac1] acs]; simpl; auto.
+    constructor; auto.
+      destruct ac1; simpl; auto.
+      destruct v as [vid|]; simpl; auto.
+      destruct_if; simpl.
+        unfold used_in_action in Hnuse.
+        destruct ac0; inv Hsome; auto.     
+
+        destruct_dec.
+Qed.
+
+Definition actions_imply (acs1 acs2:AssocList action) : Prop :=
+forall vl1 al1 v1 v2
+  (Hw: D_walk (avertexes acs1) (aarcs acs1) v1 v2 vl1 al1),
+  exists vl2, exists al2, 
+    D_walk (avertexes acs2) (aarcs acs2) v1 v2 vl2 al2.
+
+Lemma D_walk_weakening: forall A x y vl al (v1 v2:@V_set A) (a1 a2:@A_set A)
+  (H1: forall z, In z (x::vl) -> v1 z)
+  (H2: forall z, In z al -> a1 z)
+  (J: @D_walk A v2 a2 x y vl al),
+  D_walk v1 a1 x y vl al.
+Proof.
+  intros.
+  induction J; constructor.
+    apply H1; simpl; auto.
+    apply IHJ.
+      intros. apply H1. simpl; auto.
+      intros. apply H2. simpl; auto.
+    apply H1; simpl; auto.
+    apply H2; simpl; auto.
+Qed.
+
+(*
+   There is a path from x0 to y0.
+   We partition the path by the edge (z0, v0) in the following.
+   o fine if the path is empty
+   o the path (except the end) does not contain (z0,v0).
+   o otherwise
+      x0 .. z0 v0 .. z0 v0 ... ... ... z0 v0 ... y0
+*)
+Inductive wf_edge_dwalks (v:V_set) (a:A_set) 
+  (vl: @V_list value) (al: @A_list value) (x0 y0 z0 v0:@Vertex value) 
+  : list (@V_list value * @A_list value) -> Prop :=
+| WEDW_nil : 
+    x0 = y0 -> vl = V_nil -> al = A_nil ->
+    wf_edge_dwalks v a vl al x0 y0 z0 v0 nil
+| WEDW_single :
+    D_walk v a x0 y0 vl al ->
+    vl <> V_nil ->
+    ~ In (A_ends z0 v0) al ->
+    wf_edge_dwalks v a vl al x0 y0 z0 v0 [(vl, al)]
+| WEDW_more : forall vl1 al1 vals2 vl3 al3,
+    (* head *)
+    D_walk v a x0 z0 vl1 al1 ->
+    D_walk v a z0 v0 [v0] [A_ends z0 v0] ->
+    ~ In (A_ends z0 v0) al1 ->
+    (* middles *)
+    Forall (fun val2 => 
+            let '(vl2, al2) := val2 in 
+            D_walk v a v0 z0 vl2 al2 /\
+            D_walk v a z0 v0 [v0] [A_ends z0 v0] /\
+           ~ In (A_ends z0 v0) al2) vals2 ->
+    (* end *)
+    D_walk v a v0 y0 vl3 al3 ->    
+    ~ In (A_ends z0 v0) al3 ->
+    (* sum *)
+    fold_left (fun acc val2 => 
+               let '(vl2, al2) := val2 in 
+               acc ++ vl2 ++ [v0]) vals2 (vl1 ++ [v0]) ++ vl3 = vl ->
+    fold_left (fun acc val2 => 
+               let '(vl2, al2) := val2 in 
+               acc ++ al2 ++ [A_ends z0 v0]) 
+      vals2 (al1 ++ [A_ends z0 v0]) ++ al3 = al ->
+    wf_edge_dwalks v a vl al x0 y0 z0 v0 
+      ((vl1, al1) :: vals2 ++ [(vl3, al3)])
+.
+
+Lemma generate_connected_edge_dwalks: forall acs x0 y0 vl al z0 v0,
+  D_walk (avertexes acs) (aarcs acs) x0 y0 vl al ->
+  exists wks, 
+    wf_edge_dwalks (avertexes acs) (aarcs acs) vl al x0 y0 z0 v0 wks.
+Admitted.
+
+Lemma actions_len_imply_weakening: forall acs1 acs2 
+  (Hinc: actions_len_imply acs1 acs2) acs, 
+  actions_len_imply (acs++acs1) (acs++acs2).
+Proof.
+  induction acs as [|[id0 ac0] acs]; auto.
+  unfold actions_len_imply in *.
+  intros. simpl_env in *.
+  remember (action2value ac0) as ov0.
+  destruct ov0 as [v0|].
+  Case "1".
+    apply generate_connected_edge_dwalks with (z0:=index (value_id id0))
+      (v0:=index v0) in Hw.
+    destruct Hw as [wks Hw].
+    admit.
+  Case "2".
+    admit.
+Qed.
+
+Lemma actions_eq_weakening: forall acs1 acs2 (Hinc: actions_eq acs1 acs2) acs
+  (Huniq1: uniq (acs++acs1)) (Huniq2: uniq (acs++acs2)), 
+  actions_eq (acs++acs1) (acs++acs2).
+(* similar to actions_len_imply_weakening *)
+Admitted.
+
+Lemma acyclic_actions_weakening: forall acs1 acs2 
+  (Hinc: actions_len_imply acs2 acs1) acs
+  (Hacyc: acyclic_actions (acs++acs1)), acyclic_actions (acs++acs2).
+Proof.
+  intros.
+  apply actions_len_imply_weakening with (acs:=acs) in Hinc.
+  unfold acyclic_actions. intros.
+  apply Hinc in Hcyc.
+  destruct Hcyc as [vl2 [al2 [Hw Hlen]]].
+  apply Hacyc in Hw.
+  subst.
+  eapply len_le_zero__nil; eauto.
+Qed.
+
+Lemma actions_eq_nil: actions_eq nil nil.
+Admitted.
+
+Lemma actions_eq_trans: forall acs1 acs2 acs3, 
+  actions_eq acs1 acs2 -> actions_eq acs2 acs3 -> actions_eq acs1 acs3.
+Admitted.
+
+Lemma actions_eq_strenthening: forall acs acs1 acs2,
+  actions_eq (acs++acs1) (acs++acs2) ->
+  actions_eq acs1 acs2.
+Admitted.
+
+Lemma acyclic_actions_strengthening: forall acs1 acs2,
+  acyclic_actions (acs1++acs2)->
+  acyclic_actions acs2.
+Admitted.
+
+Definition substs_actions_eq_prop (n:nat) := forall acs
+  (Hlen: (length acs = n)%nat) (Huniq: uniq acs) 
+  (Hacyc: acyclic_actions acs),
+  actions_eq acs (substs_actions acs).
+
+Lemma substs_actions_eq_aux: forall n,
+  substs_actions_eq_prop n.
+Proof.
+  intro n.
+  elim n using (well_founded_induction lt_wf).
+  intros x Hrec.
+  unfold substs_actions_eq_prop in *; intros.
+  destruct acs as [|[id0 ac0] acs].
+  Case "1".
+    unfold_substs_actions.
+    apply actions_eq_nil; auto.
+  Case "2".
+    unfold_substs_actions.
+    assert (Hacyc':=Hacyc).
+    apply subst_actions_acyclic with (id0:=id0)(ac0:=ac0) in Hacyc'; 
+      simpl; auto.
+    assert (Huniq':=Huniq).
+    assert (J:=Huniq').
+    apply subst_actions_eq with (id0:=id0)(ac0:=ac0) in J; simpl; auto.
+    simpl_env in *.
+    unfold ListComposedPass.subst_actions in *.
+    remember (action2value ac0) as ov0.
+    destruct ov0 as [v0|].
+    SCase "2.1".
+      simpl in *.
+      assert (match ac0 with
+              | AC_remove => ac0
+              | AC_vsubst v1 => AC_vsubst (v1 {[v0 // id0]})
+              | AC_tsubst _ => ac0
+              end = ac0) as EQ. admit.
+      rewrite EQ in *. 
+      simpl_env in *.
+      remember (ListMap.map
+                (fun ac : action =>
+                 match ac with
+                 | AC_remove => ac
+                 | AC_vsubst v1 => AC_vsubst (v1 {[v0 // id0]})
+                 | AC_tsubst _ => ac
+                 end) acs) as acs'.
+      assert (uniq ([(id0, ac0)] ++ acs')) as Huniq''.
+        admit.
+      assert (uniq ([(id0, ac0)] ++ substs_actions acs')) as Huniq'''.
+        admit.
+      apply actions_eq_trans with (acs2:=[(id0, ac0)] ++ acs').
+      SSCase "2.1.1".
+        apply actions_eq_weakening; auto.
+        apply actions_eq_strenthening in J; auto.
+      SSCase "2.1.2".
+        apply actions_eq_weakening; auto.
+        eapply Hrec; eauto.
+        SSSCase "2.1.2.1.1".
+          admit. (* length *)
+        SSSCase "2.1.2.1.2".
+          solve_uniq.
+        SSSCase "2.1.2.1.3".
+          apply acyclic_actions_strengthening in Hacyc'; auto.
+    SCase "2.2".
+      apply actions_eq_weakening; auto.
+      SSCase "2.2.1".
+        eapply Hrec; eauto.
+          admit. (* length *)
+          solve_uniq.
+          apply acyclic_actions_strengthening in Hacyc; auto.
+      SSCase "2.2.2".
+        admit. (* uniq *)
+Qed.
+
+Lemma substs_actions_eq: forall acs (Huniq: uniq acs) 
+  (Hacyc: acyclic_actions acs), 
+  actions_eq acs (substs_actions acs).
+Proof.
+  intros.
+  assert (J:=@substs_actions_eq_aux (length acs)).
+  unfold substs_actions_eq_prop in J.
+  auto.
+Qed.
+
 (***************************************************************)
 (* Given acyclic and unique actions, the two composed passes are equivalent. *)
 Lemma list_compose_actions__list_composed_substs: forall actions 
